src/OpalUtil.v
@@ -1,0 +1,85 @@
+Require Import FMapList String OrderedTypeEx CpdtTactics.
+
+Fixpoint string_lt (l r: string) : Prop :=
+  match l, r with
+  | EmptyString, EmptyString => Logic.False
+  | EmptyString, _ => Logic.True
+  | String lh lr, String rh rr =>
+    match Compare_dec.lt_eq_lt_dec (Ascii.nat_of_ascii lh) (Ascii.nat_of_ascii rh) with
+    | inleft (left _) => Logic.True
+    | inleft (right _) => string_lt lr rr
+    | inright _ => Logic.False
+    end
+  | _, _ => Logic.False
+  end.
+
+Module String_as_OT <: UsualOrderedType.
+  Definition t := string.
+
+  Definition eq := @eq string.
+  Definition eq_refl := @eq_refl t.
+  Definition eq_sym := @eq_sym t.
+  Definition eq_trans := @eq_trans t.
+
+  Definition lt := string_lt.
+
+  Lemma lt_trans : forall x y z : t, string_lt x y -> string_lt y z -> string_lt x z.
+  Proof.
+    intros x.
+    induction x; intros ; destruct z; destruct y; try solve [inversion H] ; auto.
+    specialize IHx with y z.
+    unfold string_lt in *.
+    fold string_lt in *.
+    do 3 (edestruct Compare_dec.lt_eq_lt_dec ;
+          try (destruct s, s0) ;
+          intuition).
+  Qed.
+
+  Lemma lt_not_eq : forall x y : t, string_lt x y -> ~ eq x y.
+  Proof.
+    intros x.
+    induction x ; destruct y ; crush.
+    edestruct Compare_dec.lt_eq_lt_dec; crush.
+    unfold eq in H0.
+    destruct s. crush.
+    specialize IHx with y.
+    crush.
+  Qed.
+
+  Definition compare x y : OrderedType.Compare string_lt eq x y.
+  Proof.
+    generalize y.
+    clear y.
+    induction x; intros.
+    * destruct y.
+      - assert (eq "" "").
+        crush.
+        constructor 2. auto.
+      - constructor 1. crush.
+    * destruct y.
+      - constructor 3. crush.
+      - remember (Ascii.nat_of_ascii a) as an.
+        remember (Ascii.nat_of_ascii a0) as a0n.
+        specialize Ascii.ascii_nat_embedding with a.
+        specialize Ascii.ascii_nat_embedding with a0.
+        intros.
+        specialize IHx with y.
+        destruct Compare_dec.lt_eq_lt_dec with an a0n ;
+          try (destruct s) ;
+          inversion IHx;
+          [> constructor 1 ..
+          | constructor 2
+          | constructor 3
+          | constructor 3
+          | constructor 3
+          | constructor 3 ] ;
+          crush ;
+          edestruct Compare_dec.lt_eq_lt_dec;
+          crush.
+  Qed.
+
+  Definition eq_dec := string_dec.
+End String_as_OT.
+
+Module StringPair_OT := PairOrderedType String_as_OT String_as_OT.
+Module StringPairMap := FMapList.Make(StringPair_OT).
